theories/lang/cpp/arith/operator.v
@@ -9,13 +9,13 @@
  *)
 
 From bedrock.prelude Require Import base numbers.
-From bedrock.lang.cpp.arith Require Import types.
+Require Import bedrock.lang.prelude.platform.
 
 #[local] Open Scope Z_scope.
 
 (** truncation (used for unsigned operations) *)
 Definition trim (w : N) (v : Z) : Z :=
-  v mod (2 ^ Z.of_N w).
+  v mod (2 ^ w).
 
 Lemma trim_0_l:
   forall (v: Z),
@@ -33,17 +33,10 @@ Proof.
   by rewrite Zmod_mod.
 Qed.
 
-(** [to_unsigned sz z] is used when C++ converts signed values to unsigned
-    values.
-
-    "the unique value congruent to [z] modulo [2^sz]
-     where [sz] is the number of bits in the return type"
- *)
 Notation to_unsigned_bits := (trim) (only parsing).
-Notation to_unsigned a    := (to_unsigned_bits (bitsN a)) (only parsing).
 
-Definition bitFlipZU (len : bitsize) (z : Z) : Z :=
-  to_unsigned len (Z.lnot z).
+Definition bitFlipZU (len : N) (z : Z) : Z :=
+  to_unsigned_bits len (Z.lnot z).
 
 Lemma to_unsigned_bits_id : forall z (bits : N),
     0 <= z < 2 ^ (Z.of_N bits) ->
@@ -53,17 +46,27 @@ Proof.
   intros. rewrite Z.mod_small; auto.
 Qed.
 
-Lemma to_unsigned_id : forall z (sz : bitsize),
-    0 <= z < 2^bitsZ sz ->
-    to_unsigned sz z = z.
-Proof. destruct sz; apply to_unsigned_bits_id. Qed.
-
 Lemma to_unsigned_bits_eq : forall z (bits: N),
     to_unsigned_bits bits z = trim bits z.
 Proof. reflexivity. Qed.
 
+(** END GENERIC STUFF *)
+
+(** [to_unsigned sz z] is used when C++ converts signed values to unsigned
+    values.
+
+    "the unique value congruent to [z] modulo [2^sz]
+     where [sz] is the number of bits in the return type"
+ *)
+Notation to_unsigned a    := (to_unsigned_bits (bitsN a)) (only parsing).
+
+Lemma to_unsigned_id : forall z (sz : bitsize),
+    0 <= z < 2^platform.bitsN sz ->
+    to_unsigned sz z = z.
+Proof. destruct sz; apply to_unsigned_bits_id. Qed.
+
 Lemma to_unsigned_eq : forall z (sz : bitsize),
-    to_unsigned sz z = trim (bitsN sz) z.
+    to_unsigned sz z = trim (platform.bitsN sz) z.
 Proof. reflexivity. Qed.
 
 (** [to_signed sz z] is used when C++ converts unsigned values to signed values.
@@ -85,8 +88,8 @@ Definition to_signed_bits (bits: N) (z: Z): Z :=
 Definition to_signed (sz: bitsize) (z: Z): Z :=
   Unfold to_signed_bits (to_signed_bits (bitsN sz) z).
 
-Local Transparent bitsZ bitsN.
-Arguments bitsZ !_/.
+#[local] Transparent (* bitsZ *) bitsN.
+(* Arguments bitsZ !_/. *)
 Arguments Z.of_N !_/.
 Arguments bitsN !_/.
 
@@ -105,7 +108,7 @@ Proof.
 Qed.
 
 Lemma to_signed_id : forall (z : Z) (n : bitsize),
-  0 <= z < 2^(bitsZ n - 1) -> to_signed n z = z.
+  0 <= z < 2^(bitsN n - 1) -> to_signed n z = z.
 Proof. destruct n; apply to_signed_bits_id. Qed.
 
 Lemma to_signed_bits_neg: forall (z: Z) (bits: N),
@@ -129,10 +132,12 @@ Proof.
       rewrite Z.pow_succ_r; lia.
 Qed.
 
+(* TODO: used in bhv
 Lemma to_signed_neg : forall x (n : bitsize),
-    2^(bitsZ n - 1) - 1 < x < 2^bitsZ n ->
-    to_signed n x = trim (bitsN n) (x - 2^(bitsZ n - 1)) + - 2^(bitsZ n - 1).
+    2^(bitsN n - 1) - 1 < x < 2^bitsN n ->
+    to_signed n x = trim (bitsN n) (x - 2^(bitsN n - 1)) + - 2^(bitsN n - 1).
 Proof. move=> x n H; by pose proof (to_signed_bits_neg x (bitsN n) H). Qed.
+*)
 
 Lemma Z_opp1_mul_lt_ge:
   forall (n m: Z),
@@ -239,15 +244,15 @@ Qed.
 
 Lemma to_signed_unsigned_roundtrip:
   forall (bits: bitsize) (v: Z),
-    (-2^(Z.of_N (bitsN bits) - 1) <= v)%Z ->
-    (v <= 2^(Z.of_N (bitsN bits) - 1) - 1)%Z ->
+    (-2^(Z.of_N (platform.bitsN bits) - 1) <= v)%Z ->
+    (v <= 2^(Z.of_N (platform.bitsN bits) - 1) - 1)%Z ->
     to_signed bits (to_unsigned bits v) = v.
 Proof.
   intros; apply (to_signed_unsigned_bits_roundtrip (bitsN bits));
     destruct bits; simpl in *; lia.
 Qed.
 
-Local Lemma pow2Nm1gt1 {n : N} :
+#[local] Lemma pow2Nm1gt1 {n : N} :
   (0 < n)%N -> 1 <= 2^(Z.of_N n - 1).
 Proof.
   intros Hgt0.
