theories/lang/cpp/arith/types.v
@@ -4,72 +4,12 @@
  * See the LICENSE-BedRock file in the repository root for details.
  *)
 
-Require Import bedrock.prelude.base.
+Require Import bedrock.prelude.base bedrock.prelude.numbers.
+Require Export bedrock.lang.prelude.platform.
 
 #[local] Open Scope Z_scope.
 
-(* Bit-widths *)
-Variant bitsize : Set :=
-| W8
-| W16
-| W32
-| W64
-| W128.
-#[global] Instance bitsize_eq: EqDecision bitsize.
-Proof. solve_decision. Defined.
-#[global] Instance bitsize_countable : Countable bitsize.
-Proof.
-  apply (inj_countable'
-    (λ b,
-      match b with
-      | W8 => 0 | W16 => 1 | W32 => 2 | W64 => 3 | W128 => 4
-      end)
-    (λ n,
-      match n with
-      | 0 => W8 | 1 => W16 | 2 => W32 | 3 => W64 | 4 => W128
-      | _ => W8	(* dummy *)
-      end)).
-  abstract (by intros []).
-Defined.
-
-Definition bitsN (s : bitsize) : N :=
-  match s with
-  | W8   => 8
-  | W16  => 16
-  | W32  => 32
-  | W64  => 64
-  | W128 => 128
-  end.
-
-#[global] Instance bitsN_inj : Inj (=) (=) bitsN.
-Proof. red; intros x y H; by (destruct x; destruct y). Qed.
-
-Definition bitsZ (s : bitsize) : Z :=
-  Z.of_N (bitsN s).
-
-Definition bytesNat (s : bitsize) : nat :=
-  match s with
-  | W8 => 1
-  | W16 => 2
-  | W32 => 4
-  | W64 => 8
-  | W128 => 16
-  end.
-
-Definition bytesN (s : bitsize) : N :=
-  N.of_nat (bytesNat s).
-
-Definition bytesZ (s : bitsize) : Z :=
-  Z.of_N (bytesN s).
-
-Bind Scope N_scope with bitsize.
-
-Lemma of_size_gt_O w :
-  (0 < 2 ^ bitsZ w)%Z.
-Proof. destruct w; reflexivity. Qed.
-(* Hint Resolve of_size_gt_O. *)
-
-(* Signed and Unsigned *)
+(** ** Signed and Unsigned *)
 Variant signed : Set := Signed | Unsigned.
 #[global] Instance signed_eq_dec: EqDecision signed.
 Proof. solve_decision. Defined.
@@ -81,35 +21,22 @@ Proof.
   abstract (by intros []).
 Defined.
 
-Variant endian : Set := Little | Big.
-#[global] Instance endian_dec : EqDecision endian.
-Proof. solve_decision. Defined.
+(** ** Integral Types *)
+
+Lemma of_size_gt_O w : (0 < 2 ^ bitsN w)%Z.
+Proof. destruct w; reflexivity. Qed.
+(* Hint Resolve of_size_gt_O. *)
 
 Definition max_val (bits : bitsize) (sgn : signed) : Z :=
-  match bits , sgn with
-  | W8   , Signed   => 2^7 - 1
-  | W8   , Unsigned => 2^8 - 1
-  | W16  , Signed   => 2^15 - 1
-  | W16  , Unsigned => 2^16 - 1
-  | W32  , Signed   => 2^31 - 1
-  | W32  , Unsigned => 2^32 - 1
-  | W64  , Signed   => 2^63 - 1
-  | W64  , Unsigned => 2^64 - 1
-  | W128 , Signed   => 2^127 - 1
-  | W128 , Unsigned => 2^128 - 1
-  end.
+  match sgn with
+  | Signed => 2 ^ (bitsN bits - 1) - 1
+  | Unsigned => 2 ^ (bitsN bits) - 1
+  end%N.
 
 Definition min_val (bits : bitsize) (sgn : signed) : Z :=
   match sgn with
   | Unsigned => 0
-  | Signed =>
-    match bits with
-    | W8   => -2^7
-    | W16  => -2^15
-    | W32  => -2^31
-    | W64  => -2^63
-    | W128 => -2^127
-    end
+  | Signed => - (2 ^ (bitsN bits - 1))
   end.
 
 Definition bound (bits : bitsize) (sgn : signed) (v : Z) : Prop :=
